\documentclass[a4paper]{article}

\usepackage{algorithm}
\usepackage{algpseudocode}
\usepackage{tcolorbox}
\usepackage{graphicx}
\usepackage{amsmath}
\usepackage{amsfonts}
\usepackage{amsthm}

% newtheorem
\newtheorem{assumption}{Assumption}
\newtheorem{conjecture}{Conjecture}
\newtheorem{corollary}{Corollary}
\newtheorem{claim}{Claim}
\newtheorem{example}{Example}
\newtheorem{lemma}{Lemma}
\newtheorem{proposition}{Proposition}
\newtheorem{remark}{Remark}
\newtheorem{theorem}{Theorem}
\newtheorem{definition}{Definition}

\title{Concentration Inequalities}
\author{Peng Lingwei}
\begin{document}

\maketitle
\tableofcontents
\newpage

\section{Hoeffiding's Inequality}%
\label{sec:hoeffiding_s_inequality}

Consider the sum $ S_n = \sum^{n}_{i=1} X_i $ of independent random variable $ X_1, \ldots, X_n $.
Then, $ \forall s > 0 $,
\begin{align*}
    \mathbb{P}\left\{ S_n - \mathbb{E}S_n \ge t \right\}
    =& \mathbb{P} \left\{ \exp\left\{ s(S_n - \mathbb{E}S_n) \right\} \ge e^{st} \right\}\\
    \le& e^{-st}\mathbb{E}e^{s(S_n - \mathbb{E}S_n)}\\
    =& e^{-st} \prod^{n}_{i=1} \mathbb{E} e^{s(X_i - \mathbb{E}X_i)}
\end{align*}
\begin{lemma}
    For a random varialble $ X $ with $ \mathbb{E}X = 0 $ and $ a \le X \le b $ then for $ s \ge 0 $,
    \[
        \mathbb{E} e^{sX} \le e^{s^2{(b-a)}^2 / 8}
    \]
    
    \begin{proof}
        Because $ \mathbb{E}X = 0, a \le X \le b $, therefore $ a = 0 \wedge b = 0 $ or $ a < 0 \wedge b > 0 $.\\
        If $ a = 0 \wedge b = 0 $, $ \mathbb{E} e^{sX} \le e^{s^2{(b-a)}^2 / 8} = 1 $\\
        Else if $ a < 0 \wedge b > 0 $:\\
        From convexity,
        \[
            e^{sx} \le \frac{x - a}{b - a} e^{sb} + \frac{b - x}{b-a} e^{sa}
            \Rightarrow
            \mathbb{E}e^{sX} \le \frac{be^{sa} - ae^{sb}}{b-a} 
        \]
        Let $ f(s) = \ln\frac{be^{sa} - ae^{sb}}{b-a} $, we can analyse $ f(s) $.
        \begin{enumerate}
            \item $ f(0) = 0 $;
            \item $ f'(s) = \frac{abe^{sa} - abe^{sb}}{be^{sa} - ae^{sb}} = \frac{a^2/b - a}{e^{s(a-b)} - a/b} + 1 $, $ f'(0) = 0 $;
            \item $ f''(s) = - \frac{a}{b} {(a-b)}^2 \frac{e^{s(a-b)}}{{(e^{s(a-b)} - a/b)}^2} =  -\frac{a}{b} {(a-b)}^2 / \left\{ e^{s(a-b)} + \frac{a^2/b^2}{e^{s(a-b)}} - 2a/b \right\}$
            $ \le -\frac{a}{b} {(a-b)}^2 / \left\{ -4a/b\right\} = \frac{1}{4} {(a-b)}^2$
            \item $ f(s)= f(0) + f'(0)s + \frac{f''(\theta s)}{2} s^2 \le \frac{1}{8} {(a - b)}^2 s^2  $
        \end{enumerate}
    \end{proof}
\end{lemma}
\begin{align*}
    \mathbb{P}(S_n - \mathbb{E}S_n \ge t) \le& \inf_{s>0} \left( e^{-st} \prod^{n}_{i=1} e^{s^2{(b_i - a_i)}^2/8} \right)\\
    =& \inf_{s>0} \exp\left( {-st} + \frac{s^2}{8} \sum^{n}_{i=1} {{(b_i - a_i)}^2} \right)\\
    =& \exp \left( \frac{-2t^2}{\sum^{n}_{i=1} {(b_i - a_i)}^2} \right)
\end{align*}

\begin{theorem}
    \textbf{(Hoeffding's Inequality).}
    For bounded random variables $ X_i \in [a_i, b_i] $, where $ X_1, \ldots, X_n $ are independent, then
    \begin{equation}
    \mathbb{P}\left\{ S_n - \mathbb{E}S_n \ge t \right\} \le \exp \left( \frac{-2t^2}{\sum^{n}_{i=1} {(b_i - a_i)}^2}  \right)
    \end{equation}
    \begin{equation}
    \mathbb{P}\left\{ \mathbb{E}S_n - S_n \ge t \right\} \le \exp \left( \frac{-2t^2}{\sum^{n}_{i=1} {(b_i - a_i)}^2}  \right)
    \end{equation}
\end{theorem}

In PAC learning task, if $ l(h, (\vec{x}, y)) \in [0, 1] $,
\[
    \mathbb{P}\left\{ \left| L_S(h) - L_\mathcal{D}(h) \right| \ge \epsilon \right\} \le 2 \exp \left( \frac{-2\epsilon^2 m}{\frac{1}{m} \sum^{m}_{i=1} {(b_i - a_i)}^2}  \right) = 2 e^{-2\epsilon^2 m}
\]

\section{McDiarmid's Inequality}%
\label{sec:mcdiarmid_s_inequality}

\begin{theorem}
    \textbf{(McDiarmid's Inequality).}
    Consider independent random variables $ X_1, \ldots, X_n \in \mathcal{X} $, the function $ \phi $ satisfies
    \[
        \phi(x_1, \ldots, x_{i-1}, x_i, x_{i+1}, \ldots, x_n) - \phi(x_1, \ldots, x_{i-1}, {x'}_i, x_{i+1}, \ldots, x_n) \in [a_i, b_i]
    \]
    then,
    \begin{equation}
        \mathbb{P}\left\{ \phi(X_1, \ldots, X_n) - \mathbb{E} \phi \ge t \right\} \le \exp\left\{ \frac{-2t^2}{\sum^{n}_{i=1} {(a_i - b_i)}^2}  \right\}
    \end{equation}
    \begin{equation}
        \mathbb{P}\left\{ \mathbb{E}\phi - \phi(X_1, \ldots, X_n) \ge t \right\} \le \exp\left\{ \frac{-2t^2}{\sum^{n}_{i=1} {(a_i - b_i)}^2}  \right\}
    \end{equation}
    \begin{proof}
        We denote $ V_i = \mathbb{E}_{X_{i+1}, \ldots, X_n}[\phi | X_1, \ldots, X_i] - \mathbb{E}_{X_i, \ldots, X_n}[\phi | X_1, \ldots, X_{i-1}] $, then
        $ \sum^{n}_{i=1} V_i = \phi(X_1, \ldots, X_n) - \mathbb{E}_{X_1, \ldots, X_n}\phi $.\\
        \[
            L_i = \inf_x \mathbb{E}_{X_{i+1}, \ldots, X_n} [\phi | X_1, \ldots, X_{i-1}, x] - \mathbb{E}_{x_i, \ldots, X_n}[\phi | X_1, \ldots, X_{i-1}]
        \]
        \[
            U_i = \sup_x \mathbb{E}_{X_{i+1}, \ldots, X_n} [\phi | X_1, \ldots, X_{i-1}, x] - \mathbb{E}_{x_i, \ldots, X_n}[\phi | X_1, \ldots, X_{i-1}]
        \]
        Then, $ L_i \le V_i \le U_i $.Because $ L_i \ge L_i - U_i \ge a_i $ and $ U_i \le U_i - L_i \le b_i $,
        therefore $ a_i \le V_i \le b_i $.
        By Hoeffding, we have
        \[
            \mathbb{P}(\phi - \mathbb{E}\phi \ge t) \le \inf_{s > 0} e^{-st} \mathbb{E}_{X_1, \ldots, X_n} \left( \prod^{n}_{i=1} e^{sV_i} \right)
        \]
        Now, we look into $ \mathbb{E}_{X_1, \ldots, X_n} \left( \prod^{n}_{i=1} e^{sV_i} \right)$:
        \begin{align*}
            \mathbb{E}_{X_1, \ldots, X_n} \left( \prod^{n}_{i=1} e^{sV_i} \right)
            =& \mathbb{E}_{X_1, \ldots, X_{n-1}} \left( \prod^{n-1}_{i=1} e^{sV_i} \cdot \mathbb{E}_{X_n} e^{sV_n}\right)\\
            \le& \mathbb{E}_{X_1, \ldots, X_{n-1}} \left( \prod^{n-1}_{i=1} e^{sV_i} \cdot \right) e^{s^2 {(a_n - b_n)}^2 / 8}\\
            \ldots& \le \exp \left( s^2 \sum^{n}_{i=1} {(a_i - b_i)}^2/8 \right)
        \end{align*}
    \end{proof}
\end{theorem}
\end{document}

